secure_api/hkdf/Crypto.HMAC.fsti
@@ -7,20 +7,18 @@ module Crypto.HMAC
 
 open Crypto.Hash 
 
-open FStar.Integers 
-
 type bseq = Seq.seq UInt8.t 
 let lbseq (l:nat) = b:bseq {Seq.length b = l}
 
-let keysized (a:alg13) (l:nat) = l <= maxLength a /\ l + blockLength a < pow2 32
+let keysized (a:alg13) (l:nat) =
+  l <= maxLength a /\ 
+  l + blockLength a < pow2 32
 
 (* ghost specification; the algorithmic definition is given in the .fst *)
 noextract val hmac: 
   a: alg13 ->
-  key: bseq {keysized a (Seq.length key)} ->
-  data: bseq {
-    let l: nat = Seq.length data in 
-    l + blockLength a <= maxLength a } ->
+  key: bseq{ keysized a (Seq.length key) } ->
+  data: bseq{ Seq.length data + blockLength a <= maxLength a } ->
   lbseq (tagLength a)
 
 open FStar.HyperStack.All
@@ -28,23 +26,21 @@ open FStar.Buffer
 
 #reset-options "--max_fuel 0  --z3rlimit 20"
 (* implementation, relying on 3 variants of SHA2 supported by HACL*; 
-   we tolerate overlaps between tag and data.
+   we tolerate overlaps between tag and data. 
+   (we used to require [disjoint data tag])
 *)
 val compute:
   a: alg13 ->
   tag: lbptr (tagLength a) ->
-  key: bptr {keysized a (length key) /\ disjoint key tag} -> 
-  keylen: UInt32.t {UInt32.v keylen = length key} ->
-  data: bptr {
-    let l: nat = length data in
-    l + blockLength a < pow2 32 /\ disjoint data tag} ->
-  datalen: UInt32.t {UInt32.v datalen = length data} -> 
+  key: bptr{ keysized a (length key) /\ disjoint key tag } -> 
+  keylen: UInt32.t{ UInt32.v keylen = length key } ->
+  data: bptr{ length data + blockLength a < pow2 32 } ->
+  datalen: UInt32.t{ UInt32.v datalen = length data } -> 
   Stack unit
   (requires (fun h0 -> live h0 tag /\ live h0 key /\ live h0 data))
   (ensures  (fun h0 _ h1 -> 
     live h1 tag /\ live h0 tag /\
     live h1 key /\ live h0 key /\
     live h1 data /\ live h0 data /\ // modifies_1 tag h0 h1 /\
-    ( let l: nat = length data in 
-      l + blockLength a <= maxLength a /\ (* required for subtyping the RHS below *)    
+    ( length data + blockLength a <= maxLength a /\ (* required for subtyping the RHS below *)    
       as_seq h1 tag = hmac a (as_seq h0 key) (as_seq h0 data))))
